Updated:
* .ec files in common to changes in EasyCrypt module restriction
  syntax

* EasyCrypt source used by ucdsl implementation to the current release
  of EasyCrypt (which now has the new cost model)

uc-dsl/ucdsl-proj/src/ecCommands.mli
@@ -109,4 +109,3 @@ val ucdsl_new : unit -> unit
 (* end scope, reverting to saved one from stack, which is updated to
    include required theories of ended scope *)
 val ucdsl_end : unit -> unit
-
